Only exponent remain to be defined and his spec proved in NTT5

proof/correctness/NTT_Fq.ec
@@ -315,7 +315,29 @@ theory NTTequiv.
       op  CR.invr  <- ZModField.inv,
     pred  CR.unit  <- ZModField.unit.
 
-  op zeta1_ = ZModpRing.ofint 17.
+  op zeta1 = ZModpRing.ofint 17.
+
+  lemma exp_zeta1_128 : exp zeta1 128 = -ZModField.one.
+  proof.
+    admit.
+  qed.
+
+  lemma exp_zeta1_256 : exp zeta1 256 = ZModField.one.
+  proof.
+    admit.
+  qed.
+
+  op zetasctr_ntt5 len start = (start * 2 + 1) * (64 %/ len).
+
+  lemma zetasctr_ntt5_ge0 len start :
+    0 <= len =>
+    0 <= start =>
+    0 <= zetasctr_ntt5 len start.
+  proof.
+    move => le0len le0start; rewrite /zetasctr_ntt5.
+    apply/mulr_ge0; first by apply/addr_ge0 => //; apply mulr_ge0.
+    by move: le0len => [lt0len|//=]; apply/divz_ge0.
+  qed.
 
   module NTT5 = {
     proc ntt(r : zmod Array256.t) : zmod Array256.t = {
@@ -327,9 +349,8 @@ theory NTTequiv.
       while (len <= 64) {
        start <- 0;
        while(start < len) {
-          (*TODO: the value of zetasctr is suspicious*)
-          zetasctr <- (start * 2 + 1) * (64 %/ len);
-          zeta_ <- exp zeta1_ zetasctr;
+          zetasctr <- zetasctr_ntt5 len start;
+          zeta_ <- exp zeta1 zetasctr;
           j <- 0;
           while (j < 256) {
             t <- zeta_ * r.[bitrev 8 (j + len + start)];
@@ -356,7 +377,7 @@ theory NTTequiv.
         start <- 0;
         while(start < 256) {
           zetasctr <- bitrev 8 ((256 %/ len) + (start %/ len));
-          zeta_ <- exp zeta1_ zetasctr;
+          zeta_ <- exp zeta1 zetasctr;
           j <- 0;
           while (j < len) {
             t <- zeta_ * r.[j + len + start];
@@ -484,30 +505,526 @@ theory NTTequiv.
   (*- one that gives a postcondition when the loop being adressed is a for loop*)
   (*- another that does the same for the specific for loops that always write on different parts of the memory that is described in the postcondition (the two innermost loops in our case)*)
 
+  abbrev set2_add_mulr (p : zmod Array256.t, z : zmod, a b : int) =
+    (p.[b <- p.[a] + - z * p.[b]].[a <- p.[b <- p.[a] + - z * p.[b]].[a] + z * p.[b]])%CR.
+
+  lemma set2_add_mulr_eq1iE (p : zmod Array256.t, z : zmod, a b x : int) :
+    a <> b =>
+    a \in range 0 256 =>
+    x = a =>
+    (set2_add_mulr p z a b).[x] = (p.[a] + z * p.[b])%CR.
+  proof. by move => ? /mem_range ? ?; rewrite set_eqiE ?set_neqiE. qed.
+
+  lemma set2_add_mulr_eq2iE (p : zmod Array256.t, z : zmod, a b x : int) :
+    a <> b =>
+    b \in range 0 256 =>
+    x = b =>
+    (set2_add_mulr p z a b).[x] = (p.[a] + - z * p.[b])%CR.
+  proof. by move => ? /mem_range ? eqxb; rewrite set_neqiE ?set_eqiE // eqxb eq_sym. qed.
+
+  lemma set2_add_mulr_neqiE (p : zmod Array256.t, z : zmod, a b x : int) :
+    x <> a =>
+    x <> b =>
+    (set2_add_mulr p z a b).[x] = p.[x].
+  proof. by move => ? ?; rewrite !set_neqiE. qed.
+
   abbrev index (len start bsj : int) = bitrev 8 (bsj * len + start).
+
+  lemma index_range (k start bsj : int) :
+    k \in range 0 8 =>
+    start \in range 0 (2 ^ k) =>
+    bsj \in range 0 (2 ^ (8 - k)) =>
+    bsj * (2 ^ k) + start \in range 0 256.
+  proof.
+    move => /mem_range [? ?] Hstart_range Hbsj_range.
+    move: (range_mul_add _ _ _ _ _ Hbsj_range Hstart_range) => /=.
+    apply range_incl => //.
+    by rewrite -exprD_nneg -?addrA ?subr_ge0 //= ltzW.
+  qed.
+
+  lemma index_range_k (k start bsj : int) :
+    k \in range 0 7 =>
+    start \in range 0 (2 ^ k) =>
+    bsj \in range 0 (2 ^ (8 - k)) =>
+    bsj * (2 ^ k) + start \in range 0 256.
+  proof. by move => Hk_range; apply index_range; move: Hk_range; apply range_incl. qed.
+
+  lemma index_range_incr_k (k start bsj : int) :
+    k \in range 0 7 =>
+    start \in range 0 (2 ^ (k + 1)) =>
+    bsj \in range 0 (2 ^ (7 - k)) =>
+    bsj * (2 ^ (k + 1)) + start \in range 0 256.
+  proof.
+    move => Hk_range Hstart_range Hbsj_range; apply index_range => //.
+    + by move: (range_add _ 1 _ _ Hk_range); apply range_incl.
+    by rewrite opprD /= addrC.
+  qed.
+
+  lemma index_bijective (k start bsj x y : int) :
+    k \in range 0 8 =>
+    start \in range 0 (2 ^ k) =>
+    bsj \in range 0 (2 ^ (8 - k)) =>
+    x \in range 0 (2 ^ k) =>
+    y \in range 0 (2 ^ (8 - k)) =>
+    index (2 ^ k) x y = index (2 ^ k) start bsj <=> (x = start) /\ (y = bsj).
+  proof.
+    move => Hk_range Hstart_range Hbsj_range Hx_range Hy_range.
+    by rewrite bitrev_bijective //; [apply index_range|apply index_range|rewrite range_mul_add_eq].
+  qed.
+
+  lemma index_bijective_k (k start bsj x y : int) :
+    k \in range 0 7 =>
+    start \in range 0 (2 ^ k) =>
+    bsj \in range 0 (2 ^ (8 - k)) =>
+    x \in range 0 (2 ^ k) =>
+    y \in range 0 (2 ^ (8 - k)) =>
+    index (2 ^ k) x y = index (2 ^ k) start bsj <=> (x = start) /\ (y = bsj).
+  proof. by move => Hk_range; apply index_bijective; move: Hk_range; apply range_incl. qed.
+
+  lemma index_bijective_incr_k (k start bsj x y : int) :
+    k \in range 0 7 =>
+    start \in range 0 (2 ^ (k + 1)) =>
+    bsj \in range 0 (2 ^ (7 - k)) =>
+    x \in range 0 (2 ^ (k + 1)) =>
+    y \in range 0 (2 ^ (7 - k)) =>
+    index (2 ^ (k + 1)) x y = index (2 ^ (k + 1)) start bsj <=> (x = start) /\ (y = bsj).
+  proof.
+    move => Hk_range Hstart_range Hbsj_range Hx_range Hy_range; apply index_bijective => //.
+    + by move: (range_add _ 1 _ _ Hk_range); apply range_incl.
+    + by rewrite opprD /= addrC.
+    by rewrite opprD /= addrC.
+  qed.
+
+  lemma index_bijective_incr_k_start (k start bsj x y : int) :
+    k \in range 0 7 =>
+    start \in range 0 (2 ^ k) =>
+    bsj \in range 0 (2 ^ (7 - k)) =>
+    x \in range 0 (2 ^ (k + 1)) =>
+    y \in range 0 (2 ^ (7 - k)) =>
+    index (2 ^ (k + 1)) x y = index (2 ^ (k + 1)) start bsj <=> (x = start) /\ (y = bsj).
+  proof.
+    move => Hk_range Hstart_range; apply index_bijective_incr_k => //.
+    move: Hstart_range; apply range_incl => //.
+    apply ler_weexpn2l => //; split; first by move/mem_range: Hk_range.
+    by move => _; apply/ltzW/ltzS.
+  qed.
+
+  lemma index_bijective_incr_k_len_start (k start bsj x y : int) :
+    k \in range 0 7 =>
+    start \in range 0 (2 ^ k) =>
+    bsj \in range 0 (2 ^ (7 - k)) =>
+    x \in range 0 (2 ^ (k + 1)) =>
+    y \in range 0 (2 ^ (7 - k)) =>
+    index (2 ^ (k + 1)) x y = index (2 ^ (k + 1)) ((2 ^ k) + start) bsj <=>
+    (x = (2 ^ k) + start) /\ (y = bsj).
+  proof.
+    move => Hk_range Hstart_range Hbsj_range Hx_range Hy_range; apply index_bijective_incr_k => //.
+    rewrite (addzC _ start); move: (range_add _ (2 ^ k) _ _ Hstart_range); apply range_incl => //=.
+    + by apply expr_ge0.
+    by rewrite addr_double -exprSr //; move/mem_range: Hk_range.
+  qed.
+
+  (*TODO: define this guy such that it works.*)
+  op exponent (len start s : int) : int.
+
+  lemma exponent_0 : exponent 1 0 0 = 0.
+  proof.
+    admit.
+  qed.
+
+  lemma exponent_ge0 len start s : 0 <= exponent len start s.
+  proof.
+    admit.
+  qed.
+
+  lemma exponent_spec_00 (k start x : int) :
+    k \in range 0 7 =>
+    start \in range 0 (2 ^ k) =>
+    x \in range 0 (2 ^ k) =>
+    exp zeta1 (exponent (2 ^ k) start x) =
+    exp zeta1 (exponent (2 ^ (k + 1)) start x).
+  proof.
+    admit.
+  qed.
+
+  lemma exponent_spec_01 (k start x : int) :
+    k \in range 0 7 =>
+    start \in range 0 (2 ^ k) =>
+    x \in range 0 (2 ^ k) =>
+    exp zeta1 (zetasctr_ntt5 (2 ^ k) start + exponent (2 ^ k) start x) =
+    exp zeta1 (exponent (2 ^ (k + 1)) start (2 ^ k + x)).
+  proof.
+    admit.
+  qed.
+
+  lemma exponent_spec_10 (k start x : int) :
+    k \in range 0 7 =>
+    start \in range 0 (2 ^ k) =>
+    x \in range 0 (2 ^ k) =>
+    exp zeta1 (exponent (2 ^ k) start x) =
+    exp zeta1 (exponent (2 ^ (k + 1)) (2 ^ k + start) x).
+  proof.
+    admit.
+  qed.
+
+  lemma exponent_spec_11 (k start x : int) :
+    k \in range 0 7 =>
+    start \in range 0 (2 ^ k) =>
+    x \in range 0 (2 ^ k) =>
+    exp zeta1 (128 + zetasctr_ntt5 (2 ^ k) start + exponent (2 ^ k) start x) =
+    exp zeta1 (exponent (2 ^ (k + 1)) (2 ^ k + start) (2 ^ k + x)).
+  proof.
+    admit.
+  qed.
 
   op partial_ntt (p : zmod Array256.t, len start bsj : int) =
   BAdd.bigi
     predT
-    (fun k =>
-      (*TODO: the value of this exponent is suspicious.*)
-      (exp zeta1_ (bitrev 8 (k * start))) *
-      p.[index len k bsj])
+    (fun s =>
+      (exp zeta1 (exponent len start s)) *
+      p.[index len s bsj])
     0 len.
 
   op partial_ntt_spec (r p : zmod Array256.t, len start bsj : int) =
     r.[index len start bsj] = partial_ntt p len start bsj.
 
-  (*abbrev update (p : zmod Array256.t, k start bsj : int) =
-    p.[index (2 ^ (k + 1)) (2 ^ k + start) bsj <- ].*)
+  lemma partial_ntt_spec_k_neqxiE (r p : zmod Array256.t, k start bsj x y : int) :
+    k \in range 0 7 =>
+    start \in range 0 (2 ^ k) =>
+    bsj \in range 0 (2 ^ (7 - k)) =>
+    x \in range 0 (2 ^ k) =>
+    y \in range 0 (2 ^ (8 - k)) =>
+    x <> start =>
+    partial_ntt_spec r p (2 ^ k) x y =>
+    partial_ntt_spec
+      (set2_add_mulr r (exp zeta1 (zetasctr_ntt5 (2 ^ k) start)) (index (2 ^ (k + 1)) start bsj)
+         (index (2 ^ (k + 1)) (2 ^ k + start) bsj))
+      p (2 ^ k) x y.
+  proof.
+    move => Hk_range Hstart_range Hbsj_range Hx_range Hy_range neqxstart.
+    rewrite /partial_ntt_spec /= => <-.
+    rewrite exprS ?mulrA; first by move/mem_range: Hk_range.
+    rewrite set2_add_mulr_neqiE //.
+    + rewrite index_bijective_k => //.
+      - move: (range_mul_add _ 0 _ _ 2 Hbsj_range _); first by apply/mem_range.
+        apply range_incl => //=.
+        rewrite -exprSr; first by apply/subr_ge0/ltzW; move/mem_range: Hk_range.
+        by rewrite addrAC.
+      by rewrite negb_and; left.
+    rewrite addrA -mulrD1l.
+    rewrite index_bijective_k => //.
+    + move: (range_mul_add _ 1 _ _ 2 Hbsj_range _); first by apply/mem_range.
+      apply range_incl => //=.
+      rewrite -exprSr; first by apply/subr_ge0/ltzW; move/mem_range: Hk_range.
+      by rewrite addrAC.
+    by rewrite negb_and; left.
+  qed.
 
-(*
+  lemma partial_ntt_spec_k_neqyiE (r p : zmod Array256.t, k start bsj x y : int) :
+    k \in range 0 7 =>
+    start \in range 0 (2 ^ k) =>
+    bsj \in range 0 (2 ^ (7 - k)) =>
+    x \in range 0 (2 ^ k) =>
+    y \in range 0 (2 ^ (8 - k)) =>
+    y <> bsj * 2 =>
+    y <> bsj * 2 + 1 =>
+    partial_ntt_spec r p (2 ^ k) x y =>
+    partial_ntt_spec
+      (set2_add_mulr r (exp zeta1 (zetasctr_ntt5 (2 ^ k) start)) (index (2 ^ (k + 1)) start bsj)
+         (index (2 ^ (k + 1)) (2 ^ k + start) bsj))
+      p (2 ^ k) x y.
+  proof.
+    move => Hk_range Hstart_range Hbsj_range Hx_range Hy_range neqybsj2 neqybsj21.
+    rewrite /partial_ntt_spec /= => <-.
+    rewrite exprS ?mulrA; first by move/mem_range: Hk_range.
+    rewrite set2_add_mulr_neqiE //.
+    + rewrite index_bijective_k => //.
+      - move: (range_mul_add _ 0 _ _ 2 Hbsj_range _); first by apply/mem_range.
+        apply range_incl => //=.
+        rewrite -exprSr; first by apply/subr_ge0/ltzW; move/mem_range: Hk_range.
+        by rewrite addrAC.
+      by rewrite negb_and; right.
+    rewrite addrA -mulrD1l.
+    rewrite index_bijective_k => //.
+    + move: (range_mul_add _ 1 _ _ 2 Hbsj_range _); first by apply/mem_range.
+      apply range_incl => //=.
+      rewrite -exprSr; first by apply/subr_ge0/ltzW; move/mem_range: Hk_range.
+      by rewrite addrAC.
+    by rewrite negb_and; right.
+  qed.
 
-            t <- zeta_ * r.[bitrev 8 (j + len + start)];
-            r.[bitrev 8 (j + len + start)] <- r.[bitrev 8 (j + start)] + (-t);
-            r.[bitrev 8 (j + start)]       <- r.[bitrev 8 (j + start)] + t;
-*)
-    
+  lemma partial_ntt_spec_incr_k_neqxiE (r p : zmod Array256.t, k start bsj x y : int) :
+    k \in range 0 7 =>
+    start \in range 0 (2 ^ k) =>
+    bsj \in range 0 (2 ^ (7 - k)) =>
+    x \in range 0 (2 ^ (k + 1)) =>
+    y \in range 0 (2 ^ (7 - k)) =>
+    x <> start =>
+    x <> (2 ^ k) + start =>
+    partial_ntt_spec r p (2 ^ (k + 1)) x y =>
+    partial_ntt_spec
+      (set2_add_mulr r (exp zeta1 (zetasctr_ntt5 (2 ^ k) start)) (index (2 ^ (k + 1)) start bsj)
+         (index (2 ^ (k + 1)) (2 ^ k + start) bsj))
+      p (2 ^ (k + 1)) x y.
+  proof.
+    move => Hk_range Hstart_range Hbsj_range Hx_range Hy_range neqxstart neqxlenstart.
+    rewrite /partial_ntt_spec /= => <-.
+    rewrite set2_add_mulr_neqiE //.
+    + rewrite index_bijective_incr_k_start => //.
+      by rewrite negb_and; left.
+    rewrite index_bijective_incr_k_len_start => //.
+    by rewrite negb_and; left.
+  qed.
+
+  lemma partial_ntt_spec_incr_k_neqyiE (r p : zmod Array256.t, k start bsj x y : int) :
+    k \in range 0 7 =>
+    start \in range 0 (2 ^ k) =>
+    bsj \in range 0 (2 ^ (7 - k)) =>
+    x \in range 0 (2 ^ (k + 1)) =>
+    y \in range 0 (2 ^ (7 - k)) =>
+    y <> bsj =>
+    partial_ntt_spec r p (2 ^ (k + 1)) x y =>
+    partial_ntt_spec
+      (set2_add_mulr r (exp zeta1 (zetasctr_ntt5 (2 ^ k) start)) (index (2 ^ (k + 1)) start bsj)
+         (index (2 ^ (k + 1)) (2 ^ k + start) bsj))
+      p (2 ^ (k + 1)) x y.
+  proof.
+    move => Hk_range Hstart_range Hbsj_range Hx_range Hy_range neqybsj.
+    rewrite /partial_ntt_spec /= => <-.
+    rewrite set2_add_mulr_neqiE //.
+    + rewrite index_bijective_incr_k_start => //.
+      by rewrite negb_and; right.
+    rewrite index_bijective_incr_k_len_start => //.
+    by rewrite negb_and; right.
+  qed.
+
+  lemma IHstart_past_0 (r p : zmod Array256.t, k start bsj x y : int) :
+    k \in range 0 7 =>
+    start \in range 0 (2 ^ k) =>
+    bsj \in range 0 (2 ^ (7 - k)) =>
+    x \in range 0 start =>
+    y \in range 0 (2 ^ (7 - k)) =>
+    partial_ntt_spec r p (2 ^ (k + 1)) x y =>
+    partial_ntt_spec
+      (set2_add_mulr r (exp zeta1 (zetasctr_ntt5 (2 ^ k) start)) (index (2 ^ (k + 1)) start bsj)
+         (index (2 ^ (k + 1)) (2 ^ k + start) bsj))
+      p (2 ^ (k + 1)) x y.
+  proof.
+    move => Hk_range Hstart_range Hbsj_range Hx_range Hy_range.
+    apply partial_ntt_spec_incr_k_neqxiE => //.
+    + move: Hx_range; apply range_incl => //.
+      apply/(lez_trans (2 ^ k)); first by apply/ltzW; move/mem_range: Hstart_range.
+      apply ler_weexpn2l => //; split; first by move/mem_range: Hk_range.
+      by move => _; apply/ltzW/ltzS.
+    + by apply/ltr_eqF; move/mem_range: Hx_range.
+    by apply/ltr_eqF/ltr_paddl; [apply expr_ge0|move/mem_range: Hx_range].
+  qed.
+
+  lemma IHstart_past_1 (r p : zmod Array256.t, k start bsj x y : int) :
+    k \in range 0 7 =>
+    start \in range 0 (2 ^ k) =>
+    bsj \in range 0 (2 ^ (7 - k)) =>
+    x \in range (2 ^ k) (2 ^ k + start) =>
+    y \in range 0 (2 ^ (7 - k)) =>
+    partial_ntt_spec r p (2 ^ (k + 1)) x y =>
+    partial_ntt_spec
+      (set2_add_mulr r (exp zeta1 (zetasctr_ntt5 (2 ^ k) start)) (index (2 ^ (k + 1)) start bsj)
+         (index (2 ^ (k + 1)) (2 ^ k + start) bsj))
+      p (2 ^ (k + 1)) x y.
+  proof.
+    move => Hk_range Hstart_range Hbsj_range Hx_range Hy_range.
+    apply partial_ntt_spec_incr_k_neqxiE => //.
+    + move: Hx_range; apply range_incl => //; first by apply expr_ge0.
+      rewrite (addzC _ start); apply/ltzW.
+      move/mem_range: (range_add _ (2 ^ k) _ _ Hstart_range) => [_].
+      by rewrite addr_double -exprSr //; move/mem_range: Hk_range.
+    + apply/gtr_eqF/(ltr_le_trans (2 ^ k));first by move/mem_range: Hstart_range.
+      by move/mem_range: Hx_range.
+    by apply/ltr_eqF; move/mem_range: Hx_range.
+  qed.
+
+  lemma IHj_past_0 (r p : zmod Array256.t, k start bsj y : int) :
+    k \in range 0 7 =>
+    start \in range 0 (2 ^ k) =>
+    bsj \in range 0 (2 ^ (7 - k)) =>
+    y \in range 0 bsj =>
+    partial_ntt_spec r p (2 ^ (k + 1)) start y =>
+    partial_ntt_spec
+      (set2_add_mulr r (exp zeta1 (zetasctr_ntt5 (2 ^ k) start)) (index (2 ^ (k + 1)) start bsj)
+         (index (2 ^ (k + 1)) (2 ^ k + start) bsj))
+      p (2 ^ (k + 1)) start y.
+  proof.
+    move => Hk_range Hstart_range Hbsj_range Hy_range.
+    apply partial_ntt_spec_incr_k_neqyiE => //.
+    + move: Hstart_range; apply range_incl => //.
+      apply ler_weexpn2l => //; split; first by move/mem_range: Hk_range.
+      by move => _; apply/ltzW/ltzS.
+    + move: Hy_range; apply range_incl => //.
+      by apply/ltzW; move/mem_range: Hbsj_range.
+    by apply/ltr_eqF; move/mem_range: Hy_range.
+  qed.
+
+  lemma IHj_present_0 (r p : zmod Array256.t, k start bsj : int) :
+    k \in range 0 7 =>
+    start \in range 0 (2 ^ k) =>
+    bsj \in range 0 (2 ^ (7 - k)) =>
+    partial_ntt_spec r p (2 ^ k) start (bsj * 2) =>
+    partial_ntt_spec r p (2 ^ k) start (bsj * 2 + 1) =>
+    partial_ntt_spec
+      (set2_add_mulr r (exp zeta1 (zetasctr_ntt5 (2 ^ k) start)) (index (2 ^ (k + 1)) start bsj)
+         (index (2 ^ (k + 1)) (2 ^ k + start) bsj))
+      p (2 ^ (k + 1)) start bsj.
+  proof.
+    move => Hk_range Hstart_range Hbsj_range.
+    rewrite /partial_ntt_spec /=.
+    rewrite set2_add_mulr_eq1iE => //.
+    + rewrite index_bijective_incr_k_len_start //.
+      - move: Hstart_range; apply range_incl => //.
+        apply ler_weexpn2l => //; split; first by move/mem_range: Hk_range.
+        by move => _; apply/ltzW/ltzS.
+      by rewrite negb_and; left; apply/ltr_eqF/ltr_spaddl => //; apply/expr_gt0.
+    + by have ->:= (bitrev_range 8).
+    rewrite mulrDl -!mulrA /= -addrA.
+    rewrite -exprS; first by move/mem_range: Hk_range.
+    move => -> ->; rewrite /partial_ntt.
+    rewrite BAdd.mulr_sumr /=.
+    rewrite (BAdd.big_cat_int (2 ^ k) 0 (2 ^ (k + 1))); first by apply/expr_ge0.
+    + apply ler_weexpn2l => //; split; first by move/mem_range: Hk_range.
+      by move => _; apply/ltzW/ltzS.
+    congr.
+    + apply BAdd.eq_big_seq => x Hx_range /=.
+      rewrite -mulrA -exprS; first by move/mem_range: Hk_range.
+      congr.
+      by apply exponent_spec_00.
+    have ->: range (2 ^ k) (2 ^ (k + 1)) = map ((+)%Int (2 ^ k)) (range 0 (2 ^ k)).
+    + by rewrite -Range.range_add /= addr_double exprSr //; move/mem_range: Hk_range.
+    rewrite BAdd.big_mapT; apply BAdd.eq_big_seq => x Hx_range /=.
+    rewrite /(\o) /= mulrA -exprD_nneg.
+    + apply/zetasctr_ntt5_ge0; first by apply/expr_ge0.
+      by move/mem_range: Hstart_range.
+    + by apply/exponent_ge0.
+    rewrite !mulrDl /= -!mulrA -!addrA -!exprS.
+    + by move/mem_range: Hk_range.
+    congr.
+    by apply exponent_spec_01.
+  qed.
+
+  lemma IHj_present_1 (r p : zmod Array256.t, k start bsj : int) :
+    k \in range 0 7 =>
+    start \in range 0 (2 ^ k) =>
+    bsj \in range 0 (2 ^ (7 - k)) =>
+    partial_ntt_spec r p (2 ^ k) start (bsj * 2) =>
+    partial_ntt_spec r p (2 ^ k) start (bsj * 2 + 1) =>
+    partial_ntt_spec
+      (set2_add_mulr r (exp zeta1 (zetasctr_ntt5 (2 ^ k) start)) (index (2 ^ (k + 1)) start bsj)
+         (index (2 ^ (k + 1)) (2 ^ k + start) bsj))
+      p (2 ^ (k + 1)) (2 ^ k + start) bsj.
+  proof.
+    move => Hk_range Hstart_range Hbsj_range.
+    rewrite /partial_ntt_spec /=.
+    rewrite set2_add_mulr_eq2iE => //.
+    + rewrite index_bijective_incr_k_len_start //.
+      - move: Hstart_range; apply range_incl => //.
+        apply ler_weexpn2l => //; split; first by move/mem_range: Hk_range.
+        by move => _; apply/ltzW/ltzS.
+      by rewrite negb_and; left; apply/ltr_eqF/ltr_spaddl => //; apply/expr_gt0.
+    + by have ->:= (bitrev_range 8).
+    rewrite mulrDl -!mulrA /= -addrA.
+    rewrite -exprS; first by move/mem_range: Hk_range.
+    move => -> ->; rewrite /partial_ntt.
+    rewrite BAdd.mulr_sumr /= BAdd.sumrN /=.
+    rewrite (BAdd.big_cat_int (2 ^ k) 0 (2 ^ (k + 1))); first by apply/expr_ge0.
+    + apply ler_weexpn2l => //; split; first by move/mem_range: Hk_range.
+      by move => _; apply/ltzW/ltzS.
+    congr.
+    + apply BAdd.eq_big_seq => x Hx_range /=.
+      rewrite -mulrA -exprS; first by move/mem_range: Hk_range.
+      congr.
+      by apply exponent_spec_10.
+    have ->: range (2 ^ k) (2 ^ (k + 1)) = map ((+)%Int (2 ^ k)) (range 0 (2 ^ k)).
+    + by rewrite -Range.range_add /= addr_double exprSr //; move/mem_range: Hk_range.
+    rewrite BAdd.big_mapT; apply BAdd.eq_big_seq => x Hx_range /=.
+    rewrite /(\o) /= mulrA -exprD_nneg.
+    + apply/zetasctr_ntt5_ge0; first by apply/expr_ge0.
+      by move/mem_range: Hstart_range.
+    + by apply/exponent_ge0.
+    rewrite !mulrDl /= -!mulrA -!addrA -!exprS.
+    + by move/mem_range: Hk_range.
+    rewrite -mulNr.
+    congr.
+    rewrite -(mul1r (_ _ (_ + _)%Int)) -mulNr -exp_zeta1_128 -exprD_nneg //.
+    + apply/addr_ge0.
+     - apply/zetasctr_ntt5_ge0; first by apply/expr_ge0.
+        by move/mem_range: Hstart_range.
+      by apply/exponent_ge0.
+    rewrite addrA.
+      by apply exponent_spec_11.
+  qed.
+
+  lemma IHj_past_1 (r p : zmod Array256.t, k start bsj y : int) :
+    k \in range 0 7 =>
+    start \in range 0 (2 ^ k) =>
+    bsj \in range 0 (2 ^ (7 - k)) =>
+    y \in range 0 bsj =>
+    partial_ntt_spec r p (2 ^ (k + 1)) (2 ^ k + start) y =>
+    partial_ntt_spec
+      (set2_add_mulr r (exp zeta1 (zetasctr_ntt5 (2 ^ k) start)) (index (2 ^ (k + 1)) start bsj)
+         (index (2 ^ (k + 1)) (2 ^ k + start) bsj))
+      p (2 ^ (k + 1)) (2 ^ k + start) y.
+  proof.
+    move => Hk_range Hstart_range Hbsj_range Hy_range.
+    apply partial_ntt_spec_incr_k_neqyiE => //.
+    + rewrite (addzC _ start).
+      move: (range_add _ (2 ^ k) _ _ Hstart_range).
+      apply range_incl => /=; first by apply expr_ge0.
+      by rewrite addr_double -exprSr //; move/mem_range: Hk_range.
+    + move: Hy_range; apply range_incl => //.
+      by apply/ltzW; move/mem_range: Hbsj_range.
+    by apply/ltr_eqF; move/mem_range: Hy_range.
+  qed.
+
+  lemma IHj_future (r p : zmod Array256.t, k start bsj y : int) :
+    k \in range 0 7 =>
+    start \in range 0 (2 ^ k) =>
+    bsj \in range 0 (2 ^ (7 - k)) =>
+    y \in range ((bsj + 1) * 2) (2 ^ (8 - k)) =>
+    partial_ntt_spec r p (2 ^ k) start y =>
+    partial_ntt_spec
+      (set2_add_mulr r (exp zeta1 (zetasctr_ntt5 (2 ^ k) start)) (index (2 ^ (k + 1)) start bsj)
+         (index (2 ^ (k + 1)) (2 ^ k + start) bsj))
+    p (2 ^ k) start y.
+  proof.
+    move => Hk_range Hstart_range Hbsj_range Hy_range.
+    apply partial_ntt_spec_k_neqyiE => //.
+    + move: Hy_range; apply range_incl => //.
+      apply/mulr_ge0 => //; apply/addr_ge0 => //.
+      by move/mem_range: Hbsj_range.
+    + apply/gtr_eqF/ltzE/ltzW/ltzE; rewrite /= -mulrD1l.
+      by move/mem_range: Hy_range.
+    apply/gtr_eqF/ltzE; rewrite /= -mulrD1l.
+    by move/mem_range: Hy_range.
+  qed.
+
+  lemma IHstart_future (r p : zmod Array256.t, k start bsj x y : int) :
+    k \in range 0 7 =>
+    start \in range 0 (2 ^ k) =>
+    bsj \in range 0 (2 ^ (7 - k)) =>
+    x \in range (start + 1) (2 ^ k) =>
+    y \in range 0 (2 ^ (8 - k)) =>
+    partial_ntt_spec r p (2 ^ k) x y =>
+    partial_ntt_spec
+      (set2_add_mulr r (exp zeta1 (zetasctr_ntt5 (2 ^ k) start)) (index (2 ^ (k + 1)) start bsj)
+         (index (2 ^ (k + 1)) (2 ^ k + start) bsj))
+    p (2 ^ k) x y.
+  proof.
+    move => Hk_range Hstart_range Hbsj_range Hx_range Hy_range.
+    apply partial_ntt_spec_k_neqxiE => //.
+    + move: Hx_range; apply range_incl => //.
+      apply/addr_ge0 => //.
+      by move/mem_range: Hstart_range.
+    apply/gtr_eqF/ltzE.
+    by move/mem_range: Hx_range.
+  qed.
 
   lemma naiventt (p : zmod Array256.t) :
       hoare
@@ -549,326 +1066,50 @@ theory NTTequiv.
           (*TODO: why no simplification? Pierre-Yves*)
           rewrite lezNgt expr_gt0 //= in Hstart_range.
           rewrite /= in Hstart_range.
-          rewrite -mulrD1l !mulrA (IntID.mulrAC bsj _ 2) -mulrD1l -!mulrA.
           move: Hbsj_range.
-          rewrite -exprS; first by smt(mem_range).
           rewrite -exprSr; first by smt(mem_range).
+          rewrite -!mulrD1l.
           do 2!(rewrite mulzK ?expf_eq0 //=).
           do 2!(rewrite -divzpMr; first by apply dvdz_exp2l; smt(mem_range)).
           rewrite -exprD_subz //; [by smt(mem_range)|rewrite addrAC /=].
-          do 4!(rewrite divz_pow //=; first by smt(mem_range)).
-          rewrite mulNr opprD /= (addzC (-k)).
-          move => Hbsj_range IHstart_past_0 IHstart_past_1 IHj_past_0 IHj_past_1 IHj_future IHstart_future.
-          rewrite all_range_min in IHj_future.
+          do 3!(rewrite divz_pow //=; first by smt(mem_range)).
+          rewrite mulNr opprD /= (addzC (-k)) -!addrA.
+          move => Hbsj_range Hstart_past_0 Hstart_past_1 Hj_past_0 Hj_past_1 Hj_future Hstart_future.
+          rewrite all_range_min in Hj_future.
           + move: (range_mul_add _ 0 _ _ 2 Hbsj_range _); first by apply/mem_range.
             by move => /= /mem_range [_]; rewrite -exprSr /=; smt(mem_range).
-          rewrite all_range_min in IHj_future.
+          rewrite all_range_min in Hj_future.
           + move: (range_mul_add _ 1 _ _ 2 Hbsj_range _); first by apply/mem_range.
             by move => /= /mem_range [_]; rewrite -exprSr /=; smt(mem_range).
-          move: IHj_future => [IHj_present_0 [IHj_present_1 IHj_future]].
-          rewrite /= -mulrD1l in IHj_future.
+          move: Hj_future => [Hj_present_0 [Hj_present_1 Hj_future]].
+          rewrite /= -mulrD1l in Hj_future.
           do!split.
-          + move : IHstart_past_0 => {IHstart_past_1 IHj_past_0 IHj_past_1 IHj_present_0 IHj_present_1 IHj_future IHstart_future}.
+          + move : Hstart_past_0.
             apply all_range_imp => y Hy_range /=; apply all_range_imp => x Hx_range /=.
-            rewrite /partial_ntt_spec /= => <-.
-            rewrite !set_neqiE ?bitrev_bijective //.
-            - move: (range_incl _ _ _ 0 (2 ^ (k + 1)) _ _ Hx_range) => //.
-              * apply/(lez_trans (2 ^ k)); first by apply/ltzW; move/mem_range: Hstart_range.
-                by apply/ler_weexpn2l => //; smt(mem_range).
-              move => {Hx_range} Hx_range; move: (range_mul_add _ _ _ _ _ Hy_range Hx_range).
-              apply/range_incl => //=; rewrite -exprD_nneg //=; [by smt(mem_range)|by smt(mem_range)|].
-              by rewrite addrAC addrA /= -addrA.
-            - move: (range_incl _ _ _ 0 (2 ^ (k + 1)) _ _ Hstart_range) => //.
-              * by apply/ler_weexpn2l => //; smt(mem_range).
-              move => {Hstart_range} Hstart_range; move: (range_mul_add _ _ _ _ _ Hbsj_range Hstart_range).
-              apply/range_incl => //=; rewrite -exprD_nneg //=; [by smt(mem_range)|by smt(mem_range)|].
-              by rewrite addrAC addrA /= -addrA.
-            - rewrite range_mul_add_eq.
-              * move: Hx_range; apply/range_incl => //.
-                apply/(lez_trans (2 ^ k)); first by apply/ltzW; move/mem_range: Hstart_range.
-                by apply/ler_weexpn2l => //; smt(mem_range).
-              * move: Hstart_range; apply range_incl => //.
-                by apply/ler_weexpn2l => //; smt(mem_range).
-              by rewrite negb_and; right; apply/ltr_eqF; move/mem_range: Hx_range.
-            - move: (range_incl _ _ _ 0 (2 ^ (k + 1)) _ _ Hx_range) => //.
-              * apply/(lez_trans (2 ^ k)); first by apply/ltzW; move/mem_range: Hstart_range.
-                by apply/ler_weexpn2l => //; smt(mem_range).
-              move => {Hx_range} Hx_range; move: (range_mul_add _ _ _ _ _ Hy_range Hx_range).
-              apply/range_incl => //=; rewrite -exprD_nneg //=; [by smt(mem_range)|by smt(mem_range)|].
-              by rewrite addrAC addrA /= -addrA.
-            - move: (range_mul_add _ 1 _ _ 2 Hbsj_range _); first by apply/mem_range.
-              move => {Hbsj_range} Hbsj_range; move: (range_mul_add _ _ _ _ _ Hbsj_range Hstart_range).
-              by apply/range_incl => //=; rewrite -exprSr -?exprD_nneg //= -?addrA //=; smt(mem_range).
-            rewrite mulrDl /= -addrA -mulrA -exprS; first by move/mem_range: Hk_range.
-            rewrite range_mul_add_eq.
-            - move: Hx_range; apply/range_incl => //.
-              apply/(lez_trans (2 ^ k)); first by apply/ltzW; move/mem_range: Hstart_range.
-              by apply/ler_weexpn2l => //; smt(mem_range).
-            - rewrite (addzC _ start); move: (range_add _ (2 ^ k) _ _ Hstart_range).
-              rewrite addr_double -exprSr /=; first by move/mem_range: Hk_range.
-              by apply range_incl => //; apply expr_ge0.
-            rewrite negb_and; right; apply/ltr_eqF/ltr_paddl; first by apply/expr_ge0.
-            by move/mem_range: Hx_range.
-          + move : IHstart_past_1 => {IHstart_past_0 IHj_past_0 IHj_past_1 IHj_present_0 IHj_present_1 IHj_future IHstart_future}.
+            by apply IHstart_past_0.
+          + move : Hstart_past_1.
             apply all_range_imp => y Hy_range /=; apply all_range_imp => x Hx_range /=.
-            rewrite /partial_ntt_spec /= => <-.
-            rewrite !set_neqiE ?bitrev_bijective //.
-            - move: (range_incl _ _ _ 0 (2 ^ (k + 1)) _ _ Hx_range); first by apply/expr_ge0.
-              * rewrite exprSr -?addr_double; first by move/mem_range: Hk_range.
-                by apply/ler_add2l/ltzW; move/mem_range: Hstart_range.
-              move => {Hx_range} Hx_range; move: (range_mul_add _ _ _ _ _ Hy_range Hx_range).
-              apply/range_incl => //=; rewrite -exprD_nneg //=; [by smt(mem_range)|by smt(mem_range)|].
-              by rewrite addrAC addrA /= -addrA.
-            - move: (range_incl _ _ _ 0 (2 ^ (k + 1)) _ _ Hstart_range) => //.
-              * by apply/ler_weexpn2l => //; smt(mem_range).
-              move => {Hstart_range} Hstart_range; move: (range_mul_add _ _ _ _ _ Hbsj_range Hstart_range).
-              apply/range_incl => //=; rewrite -exprD_nneg //=; [by smt(mem_range)|by smt(mem_range)|].
-              by rewrite addrAC addrA /= -addrA.
-            - rewrite range_mul_add_eq.
-              * move: Hx_range; apply/range_incl; first by apply expr_ge0.
-                rewrite exprSr -?addr_double; first by move/mem_range: Hk_range.
-                by apply/ler_add2l/ltzW; move/mem_range: Hstart_range.
-              * move: Hstart_range; apply range_incl => //.
-                by apply/ler_weexpn2l => //; smt(mem_range).
-              by rewrite negb_and; right; apply/gtr_eqF/(ltr_le_trans (2 ^ k)); smt(mem_range).
-            - move: (range_incl _ _ _ 0 (2 ^ (k + 1)) _ _ Hx_range); first by apply expr_ge0.
-              * rewrite exprSr -?addr_double; first by move/mem_range: Hk_range.
-                by apply/ler_add2l/ltzW; move/mem_range: Hstart_range.
-              move => {Hx_range} Hx_range; move: (range_mul_add _ _ _ _ _ Hy_range Hx_range).
-              apply/range_incl => //=; rewrite -exprD_nneg //=; [by smt(mem_range)|by smt(mem_range)|].
-              by rewrite addrAC addrA /= -addrA.
-            - move: (range_mul_add _ 1 _ _ 2 Hbsj_range _); first by apply/mem_range.
-              move => {Hbsj_range} Hbsj_range; move: (range_mul_add _ _ _ _ _ Hbsj_range Hstart_range).
-              by apply/range_incl => //=; rewrite -exprSr -?exprD_nneg //= -?addrA //=; smt(mem_range).
-            rewrite mulrDl /= -addrA -mulrA -exprS; first by move/mem_range: Hk_range.
-            rewrite range_mul_add_eq.
-            - move: Hx_range; apply/range_incl; first by apply/expr_ge0.
-              rewrite exprSr -?addr_double; first by move/mem_range: Hk_range.
-              by apply/ler_add2l/ltzW; move/mem_range: Hstart_range.
-            - rewrite (addzC _ start); move: (range_add _ (2 ^ k) _ _ Hstart_range).
-              rewrite addr_double -exprSr /=; first by move/mem_range: Hk_range.
-              by apply range_incl => //; apply expr_ge0.
-            by rewrite negb_and; right; apply/ltr_eqF; move/mem_range: Hx_range.
+            by apply IHstart_past_1.
           + apply all_range_max; first by apply ltzS; move/mem_range: Hbsj_range.
-            split.
-            - move : IHj_present_0 IHj_present_1 => {IHstart_past_0 IHstart_past_1 IHj_past_0 IHj_past_1 IHj_future IHstart_future}.
-              rewrite /partial_ntt_spec /=.
-              rewrite set_eqiE // ?set_neqiE.
-              * by apply/mem_range; move: (bitrev_range 8 (bsj * (2 ^ (k + 1)) + start)).
-              * rewrite bitrev_bijective //.
-                + move: (range_incl _ _ _ 0 (2 ^ (k + 1)) _ _ Hstart_range) => //.
-                  - by apply/ler_weexpn2l => //; smt(mem_range).
-                  move => {Hstart_range} Hstart_range.
-                  move: (range_mul_add _ _ _ _ _ Hbsj_range Hstart_range).
-                  apply/range_incl => //=; rewrite -exprD_nneg //=; [by smt(mem_range)|by smt(mem_range)|].
-                  by rewrite addrAC addrA /= -addrA.
-                + move: (range_mul_add _ 1 _ _ 2 Hbsj_range _); first by apply/mem_range.
-                  move => {Hbsj_range} Hbsj_range.
-                  move: (range_mul_add _ _ _ _ _ Hbsj_range Hstart_range).
-                  apply/range_incl => //=.
-                  by rewrite -exprSr -?exprD_nneg //= -?addrA //=; smt(mem_range).
-                rewrite mulrDl /= -addrA -mulrA -exprS; first by move/mem_range: Hk_range.
-                rewrite range_mul_add_eq //=.
-                + move: Hstart_range; apply/range_incl => //.
-                  by apply/ler_weexpn2l => //; smt(mem_range).
-                + rewrite (addzC _ start); move: (range_add _ (2 ^ k) _ _ Hstart_range).
-                  rewrite addr_double -exprSr /=; first by move/mem_range: Hk_range.
-                  by apply range_incl => //; apply expr_ge0.
-                by rewrite -subr_eq /= ltr_eqF //=; apply/expr_gt0.
-              rewrite {1}exprS ?mulrA; first by move/mem_range: Hk_range.
-              move => -> ->; rewrite /partial_ntt.
-              admit.
-            move : IHj_past_0 => {IHstart_past_0 IHstart_past_1 IHj_past_1 IHj_present_0 IHj_present_1 IHj_future IHstart_future}.
-            apply all_range_imp => x Hx_range /=.
-            rewrite /partial_ntt_spec /= => <-.
-            rewrite !set_neqiE ?bitrev_bijective //.
-            - move: (range_incl _ _ _ 0 (2 ^ (k + 1)) _ _ Hstart_range) => //.
-              * by apply/ler_weexpn2l => //; smt(mem_range).
-              move => {Hstart_range} Hstart_range.
-              move: (range_mul_add _ _ _ _ _ Hx_range Hstart_range).
-              apply/range_incl => //=.
-              move/mem_range: Hbsj_range => [_ /ltzW lebsj_].
-              move: (ler_wpmul2r (2 ^ (k + 1)) _ _ _ lebsj_); first by apply/expr_ge0.
-              rewrite -exprD_nneg; [by smt(mem_range)|by smt(mem_range)|].
-              by rewrite addrAC addrA /= -addrA.
-            - move: (range_incl _ _ _ 0 (2 ^ (k + 1)) _ _ Hstart_range) => //.
-              * by apply/ler_weexpn2l => //; smt(mem_range).
-              move => {Hstart_range} Hstart_range; move: (range_mul_add _ _ _ _ _ Hbsj_range Hstart_range).
-              apply/range_incl => //=; rewrite -exprD_nneg //=; [by smt(mem_range)|by smt(mem_range)|].
-              by rewrite addrAC addrA /= -addrA.
-            - rewrite range_mul_add_eq //=.
-              * move: Hstart_range; apply/range_incl => //.
-                by apply/ler_weexpn2l => //; smt(mem_range).
-              * move: Hstart_range; apply range_incl => //.
-                by apply/ler_weexpn2l => //; smt(mem_range).
-              by apply/ltr_eqF; move/mem_range: Hx_range.
-            - move: (range_incl _ _ _ 0 (2 ^ (k + 1)) _ _ Hstart_range) => //.
-              * by apply/ler_weexpn2l => //; smt(mem_range).
-              move => {Hstart_range} Hstart_range.
-              move: (range_mul_add _ _ _ _ _ Hx_range Hstart_range).
-              apply/range_incl => //=.
-              move/mem_range: Hbsj_range => [_ /ltzW lebsj_].
-              move: (ler_wpmul2r (2 ^ (k + 1)) _ _ _ lebsj_); first by apply/expr_ge0.
-              rewrite -exprD_nneg; [by smt(mem_range)|by smt(mem_range)|].
-              by rewrite addrAC addrA /= -addrA.
-            - move: (range_mul_add _ 1 _ _ 2 Hbsj_range _); first by apply/mem_range.
-              move => {Hbsj_range} Hbsj_range; move: (range_mul_add _ _ _ _ _ Hbsj_range Hstart_range).
-              by apply/range_incl => //=; rewrite -exprSr -?exprD_nneg //= -?addrA //=; smt(mem_range).
-            rewrite mulrDl /= -addrA -mulrA -exprS; first by move/mem_range: Hk_range.
-            rewrite range_mul_add_eq.
-            - move: Hstart_range; apply/range_incl => //.
-              by apply/ler_weexpn2l => //; smt(mem_range).
-            - rewrite (addzC _ start); move: (range_add _ (2 ^ k) _ _ Hstart_range).
-              rewrite addr_double -exprSr /=; first by move/mem_range: Hk_range.
-              by apply range_incl => //; apply expr_ge0.
-            by rewrite negb_and; left; apply/ltr_eqF; move/mem_range: Hx_range.
+            split => /=.
+            - move : Hj_present_0 Hj_present_1.
+              by apply IHj_present_0.
+            move : Hj_past_0.
+            apply all_range_imp => y Hy_range /=.
+            by apply IHj_past_0.
           + apply all_range_max; first by apply ltzS; move/mem_range: Hbsj_range.
-            split.
-            - move : IHj_present_0 IHj_present_1 => {IHstart_past_0 IHstart_past_1 IHj_past_0 IHj_past_1 IHj_future IHstart_future}.
-              rewrite /partial_ntt_spec /=.
-              rewrite set_neqiE ?set_eqiE.
-              * rewrite bitrev_bijective //.
-                + rewrite (addzC _ start); move: (range_add _ (2 ^ k) _ _ Hstart_range).
-                  rewrite addr_double -exprSr /=; first by move/mem_range: Hk_range.
-                  move => {Hstart_range} Hstart_range.
-                  move: (range_incl _ _ _ 0 (2 ^ (k + 1)) _ _ Hstart_range) => //.
-                  - by apply/expr_ge0.
-                  move => {Hstart_range} Hstart_range.
-                  move: (range_mul_add _ _ _ _ _ Hbsj_range Hstart_range).
-                  apply/range_incl => //=.
-                  rewrite -exprD_nneg //=; [by smt(mem_range)|by smt(mem_range)|].
-                  by rewrite addrAC addrA /= -addrA.
-                + move: (range_incl _ _ _ 0 (2 ^ (k + 1)) _ _ Hstart_range) => //.
-                  - by apply/ler_weexpn2l => //; smt(mem_range).
-                  move => {Hstart_range} Hstart_range.
-                  move: (range_mul_add _ _ _ _ _ Hbsj_range Hstart_range).
-                  apply/range_incl => //=.
-                  rewrite -exprD_nneg //=; [by smt(mem_range)|by smt(mem_range)|].
-                  by rewrite addrAC addrA /= -addrA.
-                rewrite range_mul_add_eq //=.
-                + rewrite (addzC _ start); move: (range_add _ (2 ^ k) _ _ Hstart_range).
-                  rewrite addr_double -exprSr /=; first by move/mem_range: Hk_range.
-                  by apply range_incl => //; apply expr_ge0.
-                + move: Hstart_range; apply range_incl => //.
-                  by apply/ler_weexpn2l => //; smt(mem_range).
-                by rewrite eq_sym -subr_eq /= ltr_eqF //=; apply/expr_gt0.
-              * by apply/mem_range; move: (bitrev_range 8 ((bsj * 2 + 1) * (2 ^ k) + start)).
-              * rewrite {1}exprS ?mulrA ?addrA; first by move/mem_range: Hk_range.
-                by rewrite mulrD1l.
-              rewrite {1}exprS ?mulrA; first by move/mem_range: Hk_range.
-              move => -> ->; rewrite /partial_ntt.
-              admit.
-            move : IHj_past_1 => {IHstart_past_0 IHstart_past_1 IHj_past_0 IHj_present_0 IHj_present_1 IHj_future IHstart_future}.
-            apply all_range_imp => x Hx_range /=.
-            rewrite /partial_ntt_spec /= => <-.
-            rewrite !set_neqiE ?bitrev_bijective //.
-            - rewrite (addzC _ start); move: (range_add _ (2 ^ k) _ _ Hstart_range).
-              rewrite /= addr_double -exprSr; first by move/mem_range: Hk_range.
-              move => {Hstart_range} Hstart_range.
-              move: (range_incl _ _ _ 0 (2 ^ (k + 1)) _ _ Hstart_range) => //; first by apply expr_ge0.
-              move => {Hstart_range} Hstart_range.
-              move: (range_mul_add _ _ _ _ _ Hx_range Hstart_range).
-              apply/range_incl => //=.
-              move/mem_range: Hbsj_range => [_ /ltzW lebsj_].
-              move: (ler_wpmul2r (2 ^ (k + 1)) _ _ _ lebsj_); first by apply/expr_ge0.
-              rewrite -exprD_nneg; [by smt(mem_range)|by smt(mem_range)|].
-              by rewrite addrAC addrA /= -addrA.
-            - move: (range_incl _ _ _ 0 (2 ^ (k + 1)) _ _ Hstart_range) => //.
-              * by apply/ler_weexpn2l => //; smt(mem_range).
-              move => {Hstart_range} Hstart_range.
-              move: (range_mul_add _ _ _ _ _ Hbsj_range Hstart_range).
-              apply/range_incl => //=; rewrite -exprD_nneg //=; [by smt(mem_range)|by smt(mem_range)|].
-              by rewrite addrAC addrA /= -addrA.
-            - rewrite range_mul_add_eq //=.
-              * rewrite (addzC _ start); move: (range_add _ (2 ^ k) _ _ Hstart_range).
-                rewrite addr_double -exprSr; first by move/mem_range: Hk_range.
-                by apply/range_incl => //=; apply/expr_ge0.
-              * move: Hstart_range; apply range_incl => //.
-                by apply/ler_weexpn2l => //; smt(mem_range).
-              by rewrite negb_and; left; apply/ltr_eqF; move/mem_range: Hx_range.
-            - rewrite (addzC _ start); move: (range_add _ (2 ^ k) _ _ Hstart_range).
-              rewrite /= addr_double -exprSr; first by move/mem_range: Hk_range.
-              move => {Hstart_range} Hstart_range.
-              move: (range_incl _ _ _ 0 (2 ^ (k + 1)) _ _ Hstart_range) => //; first by apply expr_ge0.
-              move => {Hstart_range} Hstart_range.
-              move: (range_mul_add _ _ _ _ _ Hx_range Hstart_range).
-              apply/range_incl => //=.
-              move/mem_range: Hbsj_range => [_ /ltzW lebsj_].
-              move: (ler_wpmul2r (2 ^ (k + 1)) _ _ _ lebsj_); first by apply/expr_ge0.
-              rewrite -exprD_nneg; [by smt(mem_range)|by smt(mem_range)|].
-              by rewrite addrAC addrA /= -addrA.
-            - move: (range_mul_add _ 1 _ _ 2 Hbsj_range _); first by apply/mem_range.
-              move => {Hbsj_range} Hbsj_range; move: (range_mul_add _ _ _ _ _ Hbsj_range Hstart_range).
-              by apply/range_incl => //=; rewrite -exprSr -?exprD_nneg //= -?addrA //=; smt(mem_range).
-            rewrite mulrDl /= -addrA -mulrA -exprS; first by move/mem_range: Hk_range.
-            rewrite range_mul_add_eq //=.
-            - rewrite (addzC _ start); move: (range_add _ (2 ^ k) _ _ Hstart_range).
-              rewrite /= addr_double -exprSr; first by move/mem_range: Hk_range.
-              by apply/range_incl => //; apply/expr_ge0.
-            - rewrite (addzC _ start); move: (range_add _ (2 ^ k) _ _ Hstart_range).
-              rewrite /= addr_double -exprSr; first by move/mem_range: Hk_range.
-              by apply/range_incl => //; apply/expr_ge0.
-            by apply/ltr_eqF; move/mem_range: Hx_range.
-          + move : IHj_future => {IHstart_past_0 IHstart_past_1 IHj_past_0 IHj_past_1 IHj_present_0 IHj_present_1 IHstart_future}.
-            apply all_range_imp => x Hx_range /=.
-            rewrite /partial_ntt_spec /= => <-.
-            rewrite !set_neqiE ?bitrev_bijective //.
-            - move: (range_mul_add _ _ _ _ _ Hx_range Hstart_range).
-              rewrite -mulrA -exprS; first by move/mem_range: Hk_range.
-              rewrite -exprD_nneg -?addrA /=; [by smt(mem_range)|by smt(mem_range)|].
-              apply/range_incl => //; apply/mulr_ge0; last by apply/expr_ge0.
-              by apply/addr_ge0 => //; move/mem_range: Hbsj_range.
-            - move: (range_incl _ _ _ 0 (2 ^ (k + 1)) _ _ Hstart_range) => //.
-              * by apply/ler_weexpn2l => //; smt(mem_range).
-              move => {Hstart_range} Hstart_range; move: (range_mul_add _ _ _ _ _ Hbsj_range Hstart_range).
-              apply/range_incl => //=; rewrite -exprD_nneg //=; [by smt(mem_range)|by smt(mem_range)|].
-              by rewrite addrAC addrA /= -addrA.
-            - rewrite exprS ?mulrA; first by move/mem_range: Hk_range.
-              rewrite range_mul_add_eq //=.
-              apply/gtr_eqF/(ltr_le_trans ((bsj + 1) * 2)); last by move/mem_range: Hx_range.
-              by apply/ltr_pmul2r => //; apply/ltzS.
-            - move: (range_mul_add _ _ _ _ _ Hx_range Hstart_range).
-              rewrite -mulrA -exprS; first by move/mem_range: Hk_range.
-              rewrite -exprD_nneg -?addrA /=; [by smt(mem_range)|by smt(mem_range)|].
-              apply/range_incl => //; apply/mulr_ge0; last by apply/expr_ge0.
-              by apply/addr_ge0 => //; move/mem_range: Hbsj_range.
-            - move: (range_mul_add _ 1 _ _ 2 Hbsj_range _); first by apply/mem_range.
-              move => {Hbsj_range} Hbsj_range; move: (range_mul_add _ _ _ _ _ Hbsj_range Hstart_range).
-              by apply/range_incl => //=; rewrite -exprSr -?exprD_nneg //= -?addrA //=; smt(mem_range).
-            rewrite range_mul_add_eq //=.
-            apply/gtr_eqF/(ltr_le_trans ((bsj + 1) * 2)); last by move/mem_range: Hx_range.
-            by rewrite mulrDl ltzE.
-          move : IHstart_future => {IHstart_past_0 IHstart_past_1 IHj_past_0 IHj_past_1 IHj_present_0 IHj_present_1 IHj_future}.
+            split => /=.
+            - move : Hj_present_0 Hj_present_1.
+              by apply IHj_present_1.
+            move : Hj_past_1.
+            apply all_range_imp => y Hy_range /=.
+            by apply IHj_past_1.
+          + move : Hj_future.
+            apply all_range_imp => y Hy_range /=.
+            by apply IHj_future.
+          move : Hstart_future.
           apply all_range_imp => y Hy_range /=; apply all_range_imp => x Hx_range /=.
-          rewrite /partial_ntt_spec /= => <-.
-          rewrite !set_neqiE ?bitrev_bijective //.
-          + move: (range_incl _ _ _ 0 (2 ^ k) _ _ Hx_range) => //.
-            - by apply/addr_ge0 => //; move/mem_range: Hstart_range.
-            move => {Hx_range} Hx_range; move: (range_mul_add _ _ _ _ _ Hy_range Hx_range).
-            apply/range_incl => //=; rewrite -exprD_nneg //=; [by smt(mem_range)|by smt(mem_range)|].
-            by rewrite -addrA.
-          + move: (range_incl _ _ _ 0 (2 ^ (k + 1)) _ _ Hstart_range) => //.
-            - by apply/ler_weexpn2l => //; smt(mem_range).
-            move => {Hstart_range} Hstart_range; move: (range_mul_add _ _ _ _ _ Hbsj_range Hstart_range).
-            apply/range_incl => //=; rewrite -exprD_nneg //=; [by smt(mem_range)|by smt(mem_range)|].
-            by rewrite addrAC addrA /= -addrA.
-          + rewrite exprS ?mulrA; first by move/mem_range: Hk_range.
-            rewrite range_mul_add_eq //.
-            - move: Hx_range; apply/range_incl=> //.
-              by apply/addr_ge0 => //; move/mem_range: Hstart_range.
-            by rewrite negb_and; right; apply/gtr_eqF/ltzE; move/mem_range: Hx_range.
-          + move: (range_incl _ _ _ 0 (2 ^ k) _ _ Hx_range) => //.
-            - by apply/addr_ge0 => //; move/mem_range: Hstart_range.
-            move => {Hx_range} Hx_range; move: (range_mul_add _ _ _ _ _ Hy_range Hx_range).
-            apply/range_incl => //=; rewrite -exprD_nneg //=; [by smt(mem_range)|by smt(mem_range)|].
-            by rewrite -addrA.
-          + move: (range_mul_add _ 1 _ _ 2 Hbsj_range _); first by apply/mem_range.
-            move => {Hbsj_range} Hbsj_range; move: (range_mul_add _ _ _ _ _ Hbsj_range Hstart_range).
-            by apply/range_incl => //=; rewrite -exprSr -?exprD_nneg //= -?addrA //=; smt(mem_range).
-          rewrite range_mul_add_eq => //.
-          + move: Hx_range; apply/range_incl => //.
-            by apply/addr_ge0 => //; move/mem_range: Hstart_range.
-          by rewrite negb_and; right; apply/gtr_eqF/ltzE; move/mem_range: Hx_range.
+          by apply IHstart_future.
         skip.
         move => |> &hr.
         move => Hcond_len Hinv_len; move: (FOR_NAT_MUL_LE.inv_loopP _ _ _ _ _ Hcond_len Hinv_len) => //= [k [Hk_range ->>]].
@@ -880,17 +1121,17 @@ theory NTTequiv.
         rewrite /= in Hstart_range.
         rewrite -exprSr; first by smt(mem_range).
         do 2!(rewrite divz_pow //=; first by smt(mem_range)).
-        move => IHstart_past_0 IHstart_past_1 IHstart_future.
+        move => Hstart_past_0 Hstart_past_1 Hstart_future.
         do!split.
         * by apply all_range_empty.
         * by apply all_range_empty.
         * (*TODO: why can't I just apply the view all_range_min? Use rewrite.*)
           (*move: IHstart_future => /all_range_2_min.*)
-          by move: IHstart_future; rewrite all_range_2_min /=; first by smt(mem_range).
-        * by move: IHstart_future; rewrite all_range_2_min /=; first by smt(mem_range).
+          by move: Hstart_future; rewrite all_range_2_min /=; first by smt(mem_range).
+        * by move: Hstart_future; rewrite all_range_2_min /=; first by smt(mem_range).
         move => j r.
         (*TODO: the order here seems reversed...*)
-        move => {IHstart_past_0 IHstart_past_1 IHstart_future}.
+        move => {Hstart_past_0 Hstart_past_1 Hstart_future}.
         move => Hncond_j Hinv_j; move: (FOR_INT_ADD_LT.inv_outP _ _ _ _ _ Hncond_j Hinv_j);
         [by rewrite //=; apply expr_gt0|move => ->> /=].
         move => {Hncond_j Hinv_j}.
@@ -901,7 +1142,7 @@ theory NTTequiv.
         rewrite -exprD_subz //; [by smt(mem_range)|rewrite addrAC /=].
         rewrite -exprSr; first by smt(mem_range).
         rewrite (IntID.addrAC _ (-k)) /=.
-        move => IHstart_past_0 IHstart_past_1 IHj_past_0 IHj_past_1 IHj_future IHstart_future.
+        move => Hstart_past_0 Hstart_past_1 Hj_past_0 Hj_past_1 Hj_future Hstart_future.
         by rewrite addrA; split; apply/all_range_2_max => //=; smt(mem_range).
       skip.
       move => |> &hr.
@@ -922,7 +1163,7 @@ theory NTTequiv.
       rewrite lezNgt expr_gt0 //=.
       rewrite addr_double.
       rewrite -exprSr; first by smt(mem_range).
-      move => IHstart_past_0 IHstart_past_1 _.
+      move => Hstart_past_0 Hstart_past_1 _.
       apply/(all_range_2_cat _ (2 ^ k)) => //.
       by rewrite expr_ge0 //= ler_weexpn2l //; smt(mem_range).
     skip.
@@ -931,7 +1172,7 @@ theory NTTequiv.
     do!split.
     + apply all_range_2_max => //=; split; last by apply all_range_2_empty.
       apply/allP => x xinrange; rewrite /partial_ntt_spec /partial_ntt /=.
-      by rewrite BAdd.big_ltn // BAdd.big_geq //= addr0 bitrev_0 expr0 mul1r.
+      by rewrite BAdd.big_ltn // BAdd.big_geq //= addr0 exponent_0 expr0 mul1r.
     move => len r.
     by move => Hncond_len Hinv_len; move: (FOR_NAT_MUL_LE.inv_outP _ _ _ _ _ Hncond_len Hinv_len).
   qed.
@@ -940,12 +1181,13 @@ theory NTTequiv.
     ={arg} ==> ={res}.
   proof.
     proc; sp.
-  abort.
+    admit.
+  qed.
 
   op zetas_spec (zs : zmod Array128.t) =
     forall i ,
       0 <= i < 128 =>
-      zs.[i] = exp zeta1_ (bitrev 8 (i * 2)).
+      zs.[i] = exp zeta1 (bitrev 8 (i * 2)).
 
   lemma eq_NTT3_NTT4 p zs :
     zetas_spec zs =>
